

**Analysis - Exercises**  
**CHAU Dang Minh**

**Exercise 8.** Let  $(u_n)$  be a sequence defined by  $u_0 \in \mathbb{R}$  and  $u_{n+1} = u_n + e^{-u_n}$ . Show that  $u_n \rightarrow +\infty$  and

$$u_n = \ln n + \frac{\ln n}{2n} + o\left(\frac{\ln n}{n}\right).$$

*Solution.* We first show that  $u_n \rightarrow +\infty$ . For every  $n \in \mathbb{N}$ , we have  $u_{n+1} - u_n = e^{-u_n} > 0$ , or  $u_{n+1} > u_n$ . Hence  $(u_n)$  is a strictly increasing sequence. Suppose that  $(u_n)$  is bounded above by some  $M \in \mathbb{R}$ . Then, it converges to some limit  $L \in \mathbb{R}$ . Taking the limit on both sides of the recurrence relation, we get

$$L = L + e^{-L} \iff e^{-L} = 0.$$

This is a contradiction, since  $e^{-L} > 0$  for every  $L \in \mathbb{R}$ . Hence  $(u_n)$  is not bounded above, and since it is increasing, we must have  $u_n \rightarrow +\infty$ .

Let  $a_n = e^{u_n}$ , then  $a_n \rightarrow \infty$ . Also,  $u_n = \ln(a_n)$ . We have

$$a_{n+1} = e^{u_{n+1}} = e^{u_n + e^{-u_n}} = e^{u_n} e^{e^{-u_n}} = a_n e^{\frac{1}{a_n}} \geq a_n \left(1 + \frac{1}{a_n}\right) = a_n + 1.$$

Therefore,  $a_n \geq n + a_0 = n + e^{u_0} > n$  for all  $n \in \mathbb{N}$ . Since  $\frac{1}{a_n} \rightarrow 0$ , we can use the Taylor expansion of  $e^x$  at 0 to get

$$a_{n+1} = a_n \left(1 + \frac{1}{a_n} + \frac{1}{2a_n^2} + O\left(\frac{1}{a_n^3}\right)\right) = a_n + 1 + \frac{1}{2a_n} + O\left(\frac{1}{a_n^2}\right).$$

We also have

$$\begin{aligned} a_n - a_0 &= \sum_{k=0}^{n-1} (a_{k+1} - a_k) = \sum_{k=0}^{n-1} \left(1 + \frac{1}{2a_k} + O\left(\frac{1}{a_k^2}\right)\right) \\ &= n + \frac{1}{2} \sum_{k=0}^{n-1} \frac{1}{a_k} + O\left(\sum_{k=0}^{n-1} \frac{1}{a_k^2}\right) \\ &\leq n + \frac{1}{2} \sum_{k=1}^{n-1} \frac{1}{k} + \frac{1}{a_0} + O\left(\sum_{k=0}^{n-1} \frac{1}{n^2}\right) \\ &\leq n + \ln n + O(1), \end{aligned}$$

or  $a_n \leq n + \ln n + O(1)$ . Now let  $b_n = a_n - n - \frac{1}{2} \ln n$ . Then we have

$$b_{n+1} - b_n = a_{n+1} - a_n - 1 - \frac{1}{2}(\ln(n+1) - \ln n) = \frac{1}{2a_n} + O\left(\frac{1}{a_n^2}\right) - \frac{1}{2}(\ln(n+1) - \ln n).$$

Since  $\ln(n+1) - \ln n = \ln\left(1 + \frac{1}{n}\right) = \frac{1}{n} - \frac{1}{2n^2} + O\left(\frac{1}{n^3}\right)$ , we obtain

$$\begin{aligned}
b_{n+1} - b_n &= \frac{1}{2a_n} + O\left(\frac{1}{a_n^2}\right) - \frac{1}{2}\left(\frac{1}{n} - \frac{1}{2n^2} + O\left(\frac{1}{n^3}\right)\right) \\
&= \frac{1}{2}\left(\frac{1}{a_n} - \frac{1}{n}\right) + \frac{1}{4n^2} + O\left(\frac{1}{n^3} + \frac{1}{a_n^2}\right).
\end{aligned}$$

From  $a_n \leq n + \ln n + O(1)$ , for  $n \geq 1$ , we have

$$\frac{1}{a_n} \geq \frac{1}{n + \ln n + O(1)} = \frac{1}{n} \cdot \frac{1}{1 + \frac{\ln n}{n} + O\left(\frac{1}{n}\right)} = \frac{1}{n} - \frac{\ln n}{n^2} + O\left(\frac{\ln^2 n}{n^3}\right).$$

Therefore,  $0 > \frac{1}{a_n} - \frac{1}{n} > -\frac{\ln n}{n^2} + O\left(\frac{\ln^2 n}{n^3}\right)$  or  $0 < \left|\frac{1}{a_n} - \frac{1}{n}\right| < \frac{\ln n}{n^2} + O\left(\frac{\ln^2 n}{n^3}\right)$ . For some  $N_1 \in \mathbb{N}$ , we have  $\frac{\ln n}{n^2} < \frac{1}{n^{3/2}}$  for every  $n > N_1$ . Using the fact that  $\sum_{k=1}^n \frac{1}{k^p} < \infty$ , for every  $p > 1$ , we get

$$\sum_{n=1}^{\infty} \frac{\ln n}{n^2} \leq \sum_{n=1}^{N_1} \frac{\ln n}{n^2} + \sum_{n=N_1+1}^{\infty} \frac{\sqrt{n}}{n^2} = \sum_{n=1}^{N_1} \frac{\ln n}{n^2} + \sum_{n=N_1+1}^{\infty} \frac{1}{n^{3/2}} < \infty.$$

Using the same argument, we also have  $\sum_{n=1}^{\infty} O\left(\frac{\ln^2 n}{n^3}\right) < \infty$ . Hence,  $\sum_{n=1}^{\infty} \left|\frac{1}{a_n} - \frac{1}{n}\right| < \infty$ .

From the calculation of  $b_{n+1} - b_n$ , there exist  $C > 0$  and  $N_2 \in \mathbb{N}$  such that for every  $n > N_2$ , we have

$$|b_{n+1} - b_n| \leq \frac{1}{2} \left|\frac{1}{a_n} - \frac{1}{n}\right| + \frac{1}{4n^2} + C \left(\frac{1}{n^3} + \frac{1}{a_n^2}\right) < \frac{1}{2} \left|\frac{1}{a_n} - \frac{1}{n}\right| + \frac{1}{4n^2} + C \left(\frac{1}{n^3} + \frac{1}{n^2}\right).$$

Therefore,  $\sum_{n=1}^{\infty} |b_{n+1} - b_n| < \infty$ , implying that  $\sum_{n=1}^{\infty} (b_{n+1} - b_n)$  converges. Hence,  $b_n = b_0 + \sum_{k=1}^n (b_k - b_{k-1})$  converges to some limit  $b \in \mathbb{R}$ . Therefore,  $a_n = n + \frac{1}{2} \ln n + b + o(1)$ , implying that

$$u_n = \ln n + \ln \left(1 + \frac{\frac{1}{2} \ln n + b + o(1)}{n}\right).$$

Since  $\frac{\frac{1}{2} \ln n + b + o(1)}{n} \rightarrow 0$ , we can use the Taylor expansion of  $\ln(1+x)$  at 0 to get

$$u_n = \ln n + \frac{\frac{1}{2} \ln n + b + o(1)}{n} + o\left(\frac{\ln n}{2n} + \frac{b}{n} + \frac{o(1)}{n}\right) = \ln n + \frac{\ln n}{2n} + o\left(\frac{\ln n}{n}\right).$$